src/goose_lang/recovery_adequacy.v
@@ -1,0 +1,31 @@
+From iris.proofmode Require Import tactics.
+From iris.algebra Require Import auth.
+From iris.base_logic.lib Require Import proph_map.
+From iris.program_logic Require Export weakestpre adequacy.
+From Perennial.goose_lang Require Import proofmode notation.
+From Perennial.program_logic Require Import recovery_weakestpre.
+From Perennial.goose_lang Require Import typing adequacy.
+Set Default Proof Using "Type".
+
+Section recovery_adequacy.
+
+Context `{ffi_semantics: ext_semantics}.
+Context {ext_tys: ext_types ext}.
+Context `{!ffi_interp ffi}.
+
+Definition heap_namesO := leibnizO heap_names.
+Global Instance heapG_perennialG `{!heapG Σ} : perennialG heap_lang heap_crash_lang heap_namesO Σ :=
+{
+  perennial_irisG := λ Hinv hnames, @heapG_irisG _ _ _ _ _ (heap_update _ _ Hinv (@pbundleT _ _ hnames));
+  perennial_invG := λ _ _, eq_refl
+}.
+
+Section test.
+Context `{!heapG Σ}.
+
+Remark test s k Hi Hc t E (e: expr heap_lang) rec Φ Φinv Φr :
+  wpr s k Hi Hc t E e rec Φ Φinv Φr -∗ True.
+Proof. eauto. Qed.
+
+End test.
+End recovery_adequacy.
